concurrency/Modular/templates/data_struct.v
@@ -73,5 +73,6 @@ Section NodeRep.
       node_rep_R_valid_pointer: forall tp r g_in g, node_rep_R tp r g_in g |-- valid_pointer tp;
       node_rep_R_pointer_null: forall tp r g_in g, node_rep_R tp r g_in g |-- !! is_pointer_or_null tp;
       node_size: nat;
+      node_null: forall r g_info, node_rep_R nullval r g_info = !!(g_info = Some None) && seplog.emp;
   }.
 End NodeRep.
